Add inv spec

theories/syntactic.v
@@ -127,3 +127,18 @@ Proof.
   - hauto q:on use:ρ_up, T_Pi db:wf.
   - hauto q:on use:coherent_subst, T_Conv.
 Qed.
+
+Definition inv_spec Γ a A : Prop :=
+  match a with
+  | ISort Kind => False
+  | ISort Star => A ⇔ ISort Kind
+  | VarTm i => exists A0, Lookup i Γ A0 /\ A ⇔ A0
+  | Abs A0 a => exists B s1 s2, Γ ⊢ A0 ∈ ISort s1 /\ A0 :: Γ ⊢ a ∈ B /\ A0 :: Γ ⊢ B ∈ ISort s2 /\ A ⇔ Pi A0 B
+  | App b a => exists A0 B, Γ ⊢ b ∈ Pi A0 B /\ Γ ⊢ a ∈ A0 /\ A ⇔ B[a…]
+  | Pi A0 B => exists s1 s2, Γ ⊢ A0 ∈ ISort s1 /\ A0::Γ ⊢ B ∈ ISort s2 /\ A ⇔ ISort s2
+  end.
+
+Lemma wt_inv Γ a A (h : Γ ⊢ a ∈ A) : inv_spec Γ a A.
+Proof.
+  elim : Γ a A /h=>//=.
+  -
